do ex 3.4 in a new file but don't finish the sorry proofs lul

ConcreteSemanticsLean/ch3_4.lean
@@ -1,28 +1,21 @@
-import ConcreteSemanticsLean.cslib
-import Init.Prelude
-import Mathlib.Tactic.Linarith
+-- Doing this section with already defined functions was messing me up, so new file
 import Mathlib.Tactic.Ring
 import Mathlib.Tactic.Basic
 
-section ch3_prelim
-  /- Ch3.1.1, Syntax -/
-  -- Arithmetic EXPression
+section ch3_4 -- p32
   inductive aexp : Type
   | ANum    : Int → aexp
   | AString : String → aexp
   | APlus   : aexp → aexp → aexp
+  | Times   : aexp → aexp → aexp
   deriving Repr
   open aexp
 
   #eval ANum 5
   #eval AString "hello world"
   #eval APlus (AString "hello") (AString "world")
-  #eval APlus (ANum 2) (APlus (AString "hello") (ANum 3))
+  #eval APlus (ANum 2) (Times (AString "hello") (ANum 3))
 
-  /- Ch3.1.2, Semantics -/
-  -- `val` is `Int`
-  -- `vname` is `String`
-  -- `state` is `vname → val` or `String → Int`
   def state : Type := String → Int
 
   @[simp] def aval (a : aexp) (st : state) : Int :=
@@ -30,14 +23,9 @@ section ch3_prelim
     | ANum n      => n
     | AString str => st str
     | APlus a1 a2 => aval a1 st + aval a2 st
+    | Times a1 a2 => aval a1 st * aval a2 st
 
   #eval aval (APlus (ANum 3) (AString "x")) (fun _ => 0)
-
-  -- def upst (a b : Int) (u : st) :=
-  --   match a, b with
-  --   | 0, 0
-
-  -- notation "f(" a " := " b ")" => sorry
 
   /- Ch3.1.3, Constant Folding -/
   def asimp_const (a : aexp) : aexp :=
@@ -48,15 +36,28 @@ section ch3_prelim
       match asimp_const x, asimp_const y with
       | ANum x, ANum y => ANum (x + y)
       | x, y           => APlus x y
+    | Times x y =>
+      match asimp_const x, asimp_const y with
+      | ANum x, ANum y => ANum (x * y)
+      | x, y           => Times x y
 
-  #eval asimp_const (APlus (ANum 2) (ANum 3))
-  #eval asimp_const (APlus (ANum 2) (asimp_const (APlus (ANum 1) (ANum 8))))
-  #eval asimp_const (APlus (ANum 2) (asimp_const (APlus (ANum 1) (APlus (ANum 1) (ANum 8)))))
+  #eval asimp_const (Times (ANum 2) (ANum 3))
+  #eval asimp_const (APlus (ANum 2) (asimp_const (Times (ANum 2) (ANum 8))))
+  #eval asimp_const (APlus (ANum 2) (asimp_const (Times (ANum 2) (APlus (ANum 2) (ANum 8)))))
 
   theorem asimp_const_is_aval : ∀ (a : aexp) (st : state), (aval (asimp_const a) st) = (aval a st) := by
     intro a st
     induction a <;> simp
     case APlus x y ihx ihy =>
+      simp [asimp_const]
+      split
+      · case h_1 x' y' numx' numy' => -- ANum x, ANum y case
+        simp
+        simp [numx'] at ihx;
+        simp [numy'] at ihy;
+        rw [ihx, ihy]
+      · case h_2 => simp [asimp_const, ihx, ihy] -- Otherwise
+    case Times x t ihx ihy =>
       simp [asimp_const]
       split
       · case h_1 x' y' numx' numy' => -- ANum x, ANum y case
@@ -79,62 +80,51 @@ section ch3_prelim
       | _ => APlus a (ANum x)
     | a, b           => APlus a b
 
-  -- holy shit im cooking wtf !!!!!!
+  -- kyle was cooking here
   theorem aval_plus : aval (aexp_plus a b) st = aval a st + aval b st := by
     rcases a <;> rcases b <;> simp [aval, aexp_plus] <;> split <;> simp [aval] <;> ring
+
+  def aexp_times (a b : aexp) : aexp :=
+    match a, b with
+    | ANum x, ANum y => ANum (x * y)
+    | ANum x, a      =>
+      match x with
+      | 0 => ANum 0 -- 0 * a
+      | 1 => a      -- 1 * a
+      | _ => Times a (ANum x)
+    | a, ANum x      =>
+      match x with
+      | 0 => ANum 0 -- 0 * a
+      | 1 => a      -- 1 * a
+      | _ => Times a (ANum x)
+    | a, b           => Times a b
+
+  -- kyle was cooking here (i literally only did substition on his work)
+  theorem aval_times : aval (aexp_times a b) st = aval a st * aval b st := by
+    rcases a <;> rcases b <;> simp [aval, aexp_times] <;> split <;> simp [aval] <;> ring
 
   def asimp (a : aexp) : aexp :=
     match a with
     | ANum n => ANum n
     | AString x => AString x
     | APlus a b => aexp_plus (asimp a) (asimp b)
+    | Times a b => aexp_times (asimp a) (asimp b)
 
-  theorem APlus_0 : aval (APlus (ANum 0) a) st = aval a st := by rcases a <;> simp
+  theorem APlus_0 : aval (APlus (ANum 0) a) st = aval a st := by simp
+
+  theorem ATimes_0 : aval (Times (ANum 0) a) st = 0 := by simp
+
+  theorem ATimes_1 : aval (Times (ANum 1) a) st = aval a st := by simp
 
   -- might be worth trying to rewrite some of the def or removing entirely. idk how to solve!
   theorem asimp_is_asimp_const : aval (asimp a) = aval (asimp_const a) := by
     rcases a <;> simp [asimp, asimp_const, aexp_plus]
     case APlus a b => sorry
+    case Times a b => sorry
 
   theorem asimp_is_aval : aval (asimp a) st = aval a st := by
     rcases a <;> simp [aval, asimp]
     case APlus x y =>
       rcases x <;> rcases y <;> simp [aval, aexp_plus, asimp] <;> split <;> sorry
-
-  /- Ch3.2 Boolean Expressions -/
-
-end ch3_prelim
-
-section ch3_1 -- p31
-  open aexp
-  def optimal (a : aexp) : Bool :=
-    match a with
-    | APlus x y =>
-      match x, y with
-      | ANum _, ANum _  => false
-      | exp1, exp2   =>
-        match optimal exp1, optimal exp2 with
-        | true, true => true
-        | _, _ => false
-    | ANum _ => true
-    | AString _ => true
-
-  theorem asimp_const_is_optimal : optimal (asimp_const a) := by
-    induction a <;> simp [optimal, asimp_const]
-    case APlus =>
-      split
-      · case h_1 => simp [optimal] -- Adding two ANums
-      · case h_2 left right ihleft ihright _ _ _ => simp [optimal, ihleft, ihright] -- Adding two other things
-end ch3_1
-
-section ch3_2 -- p31
-end ch3_2
-
-section ch3_3 -- p31
-end ch3_3
-
-section ch3_5 -- p32
-end ch3_5
-
-section ch3_6 -- p32
-end ch3_6
+    case Times x y => sorry
+end ch3_4
